mechanization/theories/PtsSignature.v
@@ -13,8 +13,9 @@ Record PtsSig : Type :=
 Record PredicativeSig (P : PtsSig) : Type :=
   mkPredicativeSig {
       pred_rel : relation (St P);
+      pred_irrel : forall (s1 s2 : St P) (lt lt' : pred_rel s1 s2), lt = lt';
       ord_rel : order (St P) pred_rel;
       wf_rel : well_founded pred_rel;
       ord_ax : forall s1 s2 : St P, Ax P s1 s2 -> pred_rel s1 s2 /\ s1 <> s2;
-      ord_ru : forall s1 s2 s3 : St P, Ru P s1 s2 s3 -> (pred_rel s1 s3) /\ (pred_rel s1 s2);
+      ord_ru : forall s1 s2 s3 : St P, Ru P s1 s2 s3 -> (pred_rel s1 s3) /\ (pred_rel s2 s3);
     }.
